updates

intermediate/Veritas.Intermediate.Store.fst
@@ -1,4 +1,4 @@
-            module Veritas.Intermediate.Store
+module Veritas.Intermediate.Store
 open FStar.Classical
 
 let update_slot #vcfg (st:vstore_raw vcfg) (s:slot_id vcfg) (e:vstore_entry vcfg)
@@ -645,31 +645,12 @@ let bevict_from_store
                           empty_slot st' s})
   = admit()
 
-
-let store_contains_key (#vcfg:_) (st:vstore vcfg) (k:key): bool  = admit()
-
-let lemma_stored_key_implies_contains (#vcfg:_) (st: vstore vcfg) (s:inuse_slot_id st):
-  Lemma (ensures (store_contains_key st (stored_key st s)))
-  = admit()
-
-
-let slot_of_key (#vcfg:_) (st:vstore vcfg) (k:key{store_contains_key st k}): 
-  (s:inuse_slot_id st{stored_key st s = k}) = admit()
-
-let stored_value_by_key  (#vcfg:_) (st:vstore vcfg) (k:key{store_contains_key st k}) : value_type_of k
-  = admit()
-
-let add_method_of_by_key (#vcfg:_) (st:vstore vcfg) (k:key{store_contains_key st k}) : add_method
-  = admit()
-
 let pointing_slot (#vcfg:_) 
                 (st:vstore vcfg) 
                 (s:inuse_slot_id st{Root <> stored_key st s /\ add_method_of st s = Spec.MAdd})
  : Tot (s':inuse_slot_id st{points_to st s' s}) = admit()
 
-let lemma_empty_contains_nokey (#vcfg:_) (k:key):
-  Lemma (ensures (let st = empty_store vcfg in
-                  not (store_contains_key st k))) = admit()
+let as_map (#vcfg:_) (st:ismap_vstore vcfg) : Spec.vstore = admit()
 
 let lemma_ismap_update_value
       (#vcfg:_)
@@ -677,6 +658,27 @@ let lemma_ismap_update_value
       (s:inuse_slot_id st)
       (v:value_type_of (stored_key st s))
   : Lemma (ensures (is_map (update_value st s v)))
+  = admit()
+
+let lemma_ismap_madd_to_store (#vcfg:_) (st:ismap_vstore vcfg)
+  (s:empty_slot_id st)
+  (k:key) (v:value_type_of k)
+  (s':merkle_slot_id st)
+  (d:bin_tree_dir {points_to_none st s' d})
+  : Lemma (requires (not (store_contains_key st k)))
+          (ensures (is_map (madd_to_store st s k v s' d)))
+  = admit()
+
+let lemma_ismap_madd_to_store_split 
+  (#vcfg: verifier_config)
+  (st:ismap_vstore vcfg)
+  (s:empty_slot_id st)
+  (k:key) (v:value_type_of k)
+  (s':merkle_slot_id st)
+  (d:bin_tree_dir {points_to_some_slot st s' d})
+  (d2:bin_tree_dir)  
+  : Lemma (requires (not (store_contains_key st k)))
+          (ensures (is_map (madd_to_store_split st s k v s' d d2)))
   = admit()
 
 let lemma_ismap_correct (#vcfg:_) (st:ismap_vstore vcfg) (s1 s2: inuse_slot_id st)
@@ -687,55 +689,34 @@ let lemma_ismap_correct (#vcfg:_) (st:ismap_vstore vcfg) (s1 s2: inuse_slot_id s
 let lemma_empty_store_is_map (#vcfg:_):
   Lemma (ensures (is_map (empty_store vcfg))) = admit()
 
-let lemma_madd_to_store_is_map
+let lemma_empty_contains_nokey (#vcfg:_) (k:key):
+  Lemma (ensures (let st = empty_store vcfg in
+                  not (store_contains_key st k))) = admit()
+
+let lemma_madd_root_to_store_is_map
       (#vcfg:_)
       (st:ismap_vstore vcfg{not (store_contains_key st Root)}) 
       (s:empty_slot_id st) 
       (v:value_type_of Root) 
   : Lemma (ensures (is_map (madd_to_store_root st s v))) = admit()
 
-let as_map (#vcfg:_) (st:ismap_vstore vcfg) : Spec.vstore = admit()
-
 let lemma_as_map_empty (vcfg:_)
   : Lemma (ensures (let st = empty_store vcfg in
                      forall (k:key). as_map st k = None)) = admit()
 
-let lemma_as_map_slot_key_equiv (#vcfg:_) (st:ismap_vstore vcfg) (s:slot_id vcfg) (k:key)
-  : Lemma (requires (slot_key_equiv st s k)) 
-          (ensures (Spec.store_contains (as_map st) k /\
-                    stored_value st s = Spec.stored_value (as_map st) k /\
-                    add_method_of st s = Spec.add_method_of (as_map st) k))
-  = admit()
-
-let lemma_as_map_slot_key_equiv2 (#vcfg:_) (st:ismap_vstore vcfg) (s:inuse_slot_id _)
+let lemma_as_map_slot_key_equiv (#vcfg:_) (st:ismap_vstore vcfg) (s:inuse_slot_id _)
   : Lemma (ensures (let k = stored_key st s in
                     let stk = as_map st in
                     Spec.store_contains stk k /\
                     stored_value st s = Spec.stored_value stk k /\
                     add_method_of st s = Spec.add_method_of stk k)) = admit()
 
-
-let lemma_store_rel_contains_key (#vcfg:_) (st:vstore vcfg) (st':Spec.vstore) (k:key)
-  : Lemma (requires (store_rel st st'))
-          (ensures (store_contains_key st k = Spec.store_contains st' k))
-  = admit()
-
-let lemma_store_rel_stored_value (#vcfg:_) (st:vstore vcfg) (st':Spec.vstore) (k:key)
-  : Lemma (requires (store_rel st st' /\ store_contains_key st k))
-          (ensures (stored_value_by_key st k = Spec.stored_value st' k))
-  = admit()
-
-let lemma_store_rel_add_method_of (#vcfg:_) (st:vstore vcfg) (st':Spec.vstore) (k:key)
-  : Lemma (requires (store_rel st st' /\ store_contains_key st k))
-          (ensures (add_method_of_by_key st k = Spec.add_method_of st' k))
-  = admit()
-
-let lemma_store_rel_update_value (#vcfg:_) (st:vstore vcfg) (st':Spec.vstore) (s:slot_id vcfg) (k:key) (v:value_type_of k)
-  : Lemma (requires (store_rel st st' /\ slot_key_equiv st s k))
-          (ensures (store_rel (update_value st s v) (Spec.update_store st' k v)))
-  = admit()
-
-
+let slot_of_key (#vcfg:_) (st:ismap_vstore vcfg) (k: key{let stk = as_map st in
+                                                                  Spec.store_contains stk k})
+  : Tot (s: inuse_slot_id st {let stk = as_map st in
+                              k = stored_key st s /\
+                              stored_value st s = Spec.stored_value stk k /\
+                              add_method_of st s = Spec.add_method_of stk k}) = admit()
 
 (*
 (* update the data value of a data key *)
